theories/examples/sort.v
@@ -1,9 +1,9 @@
 From stdpp Require Import sorting.
 From actris.channel Require Import proto_channel proofmode.
 From iris.heap_lang Require Import proofmode notation.
-From actris.utils Require Import list compare.
+From actris.utils Require Export llist compare.
 
-Definition lmerge : val :=
+Definition lmerge : val. (*
   rec: "go" "cmp" "ys" "zs" :=
     if: lisnil "ys" then "zs" else
     if: lisnil "zs" then "ys" else
@@ -12,21 +12,20 @@ Definition lmerge : val :=
     if: "cmp" "y" "z"
     then lcons "y" ("go" "cmp" (ltail "ys") "zs")
     else lcons "z" ("go" "cmp" "ys" (ltail "zs")).
+*) Admitted.
 
 Definition sort_service : val :=
   rec: "go" "c" :=
     let: "cmp" := recv "c" in
     let: "xs" := recv "c" in
-    if: llength !"xs" ≤ #1 then send "c" #() else
-    let: "ys_zs" := lsplit !"xs" in
-    let: "ys" := ref (Fst "ys_zs") in
-    let: "zs" := ref (Snd "ys_zs") in
+    if: llength "xs" ≤ #1 then send "c" #() else
+    let: "zs" := lsplit "xs" in
     let: "cy" := start_chan "go" in
     let: "cz" := start_chan "go" in
-    send "cy" "cmp";; send "cy" "ys";;
+    send "cy" "cmp";; send "cy" "xs";;
     send "cz" "cmp";; send "cz" "zs";;
     recv "cy";; recv "cz";;
-    "xs" <- lmerge "cmp" !"ys" !"zs";;
+    lmerge "cmp" "xs" "zs";;
     send "c" #().
 
 Section sort.
@@ -37,19 +36,22 @@ Section sort.
          `{!RelDecision R, !Total R} (cmp : val),
        MSG cmp {{ cmp_spec I R cmp }};
      <!> (xs : list A) (l : loc) (vs : list val),
-       MSG #l {{ l ↦ llist vs ∗ [∗ list] x;v ∈ xs;vs, I x v }};
+       MSG #l {{ llist l vs ∗ [∗ list] x;v ∈ xs;vs, I x v }};
      <?> (xs' : list A) (vs' : list val),
        MSG #() {{ ⌜ Sorted R xs' ⌝ ∗ ⌜ xs' ≡ₚ xs ⌝ ∗
-                  l ↦ llist vs' ∗ [∗ list] x;v ∈ xs';vs', I x v }};
+                  llist l vs' ∗ [∗ list] x;v ∈ xs';vs', I x v }};
      END)%proto.
 
   Lemma lmerge_spec {A} (I : A → val → iProp Σ) (R : A → A → Prop)
-      `{!RelDecision R, !Total R} (cmp : val) xs1 xs2 vs1 vs2 :
+      `{!RelDecision R, !Total R} (cmp : val) l1 l2 xs1 xs2 vs1 vs2 :
     cmp_spec I R cmp -∗
-    {{{ ([∗ list] x;v ∈ xs1;vs1, I x v) ∗ ([∗ list] x;v ∈ xs2;vs2, I x v) }}}
-      lmerge cmp (llist vs1) (llist vs2)
-    {{{ ws, RET llist ws; [∗ list] x;v ∈ list_merge R xs1 xs2;ws, I x v }}}.
-  Proof.
+    {{{
+      llist l1 vs1 ∗ llist l2 vs2 ∗
+      ([∗ list] x;v ∈ xs1;vs1, I x v) ∗ ([∗ list] x;v ∈ xs2;vs2, I x v)
+    }}}
+      lmerge cmp #l1 #l2
+    {{{ ws, RET #(); llist l1 ws ∗ [∗ list] x;v ∈ list_merge R xs1 xs2;ws, I x v }}}.
+  Proof. (*
     iIntros "#Hcmp" (Ψ) "!> [HI1 HI2] HΨ". iLöb as "IH" forall (xs1 xs2 vs1 vs2 Ψ).
     wp_lam. wp_apply (lisnil_spec with "[//]"); iIntros (_).
     destruct xs1 as [|x1 xs1], vs1 as [|v1 vs1]; simpl; done || wp_pures.
@@ -74,7 +76,7 @@ Section sort.
       iIntros (ws) "HI".
       wp_apply (lcons_spec with "[//]"); iIntros (_).
       iApply "HΨ". iFrame.
-  Qed.
+  Qed. *) Admitted.
 
   Lemma sort_service_spec p c :
     {{{ c ↣ iProto_dual sort_protocol <++> p @ N }}}
@@ -85,14 +87,14 @@ Section sort.
     wp_lam.
     wp_recv (A I R ?? cmp) as "#Hcmp".
     wp_recv (xs l vs) as "[Hl HI]".
-    wp_load. wp_apply (llength_spec with "[//]"); iIntros (_).
+    wp_apply (llength_spec with "Hl"); iIntros "Hl".
     iDestruct (big_sepL2_length with "HI") as %<-.
     wp_op; case_bool_decide as Hlen; wp_if.
     { assert (Sorted R xs).
       { destruct xs as [|x1 [|x2 xs]]; simpl in *; eauto with lia. }
       wp_send with "[$Hl $HI]"; first by auto. by iApply "HΨ". }
-    wp_load. wp_apply (lsplit_spec with "[//]"); iIntros (vs1 vs2 ->).
-    wp_alloc l1 as "Hl1"; wp_alloc l2 as "Hl2".
+    wp_apply (lsplit_spec with "Hl"); iIntros (l2 vs1 vs2);
+      iDestruct 1 as (->) "[Hl1 Hl2]".
     iDestruct (big_sepL2_app_inv_r with "HI") as (xs1 xs2 ->) "[HI1 HI2]".
     wp_apply (start_chan_proto_spec N sort_protocol); iIntros (cy) "Hcy".
     { rewrite -{2}(right_id END%proto _ (iProto_dual _)).
@@ -106,9 +108,7 @@ Section sort.
     wp_send with "[$Hl2 $HI2]".
     wp_recv (ys1 ws1) as (??) "[Hl1 HI1]".
     wp_recv (ys2 ws2) as (??) "[Hl2 HI2]".
-    do 2 wp_load.
-    wp_apply (lmerge_spec with "Hcmp [$HI1 $HI2]"). iIntros (ws) "HI".
-    wp_store.
+    wp_apply (lmerge_spec with "Hcmp [$Hl1 $Hl2 $HI1 $HI2]"); iIntros (ws) "[Hl HI]".
     wp_send ((list_merge R ys1 ys2) ws) with "[$Hl $HI]".
     - iSplit; iPureIntro.
       + by apply (Sorted_list_merge _).
