theories/examples/sort_elem_client.v
@@ -2,21 +2,18 @@ From stdpp Require Import sorting.
 From actris.channel Require Import proto_channel proofmode.
 From iris.heap_lang Require Import proofmode notation.
 From iris.heap_lang Require Import assert.
-From actris.utils Require Import list compare.
+From actris.utils Require Import llist compare.
 From actris.examples Require Import sort_elem.
 
 Definition send_all : val :=
   rec: "go" "c" "xs" :=
-    match: "xs" with
-      SOME "p" => send "c" #cont;; send "c" (Fst "p");; "go" "c" (Snd "p")
-    | NONE => #()
-    end.
+    if: lisnil "xs" then #() else
+    send "c" #cont;; send "c" (lpop "xs");; "go" "c" "xs".
 
 Definition recv_all : val :=
   rec: "go" "c" :=
-    if: recv "c"
-    then let: "x" := recv "c" in lcons "x" ("go" "c")
-    else lnil #().
+    if: ~recv "c" then lnil #() else
+    let: "x" := recv "c" in lcons "x" ("go" "c").
 
 Definition sort_elem_client : val :=
   λ: "cmp" "xs",
@@ -30,26 +27,28 @@ Section sort_elem_client.
   Context `{!heapG Σ, !proto_chanG Σ} (N : namespace).
   Context {A} (I : A → val → iProp Σ) (R : relation A) `{!RelDecision R, !Total R}.
 
-  Lemma send_all_spec c p xs' xs vs :
-    {{{ c ↣ sort_elem_head_protocol I R xs' <++> p @ N ∗ [∗ list] x;v ∈ xs;vs, I x v }}}
-      send_all c (llist vs)
+  Lemma send_all_spec c p xs' l xs vs :
+    {{{ llist l vs ∗ c ↣ sort_elem_head_protocol I R xs' <++> p @ N ∗ [∗ list] x;v ∈ xs;vs, I x v }}}
+      send_all c #l
     {{{ RET #(); c ↣ sort_elem_head_protocol I R (xs' ++ xs) <++> p @ N }}}.
   Proof.
-    iIntros (Φ) "[Hc HI] HΦ".
+    iIntros (Φ) "(Hl & Hc & HI) HΦ".
     iInduction xs as [|x xs] "IH" forall (xs' vs); destruct vs as [|v vs]=>//.
-    { wp_lam; wp_pures. iApply "HΦ". rewrite right_id_L. iFrame. }
-    iDestruct "HI" as "[HIxv HI]". wp_lam; wp_pures.
-    wp_select. wp_send with "[$HIxv]". wp_apply ("IH" with "Hc HI").
-    by rewrite -assoc_L.
+    { wp_lam. wp_apply (lisnil_spec with "Hl"); iIntros "Hl"; wp_pures.
+      iApply "HΦ". rewrite right_id_L. iFrame. }
+    iDestruct "HI" as "[HIxv HI]". wp_lam.
+    wp_apply (lisnil_spec with "Hl"); iIntros "Hl". wp_select.
+    wp_apply (lpop_spec with "Hl"); iIntros "Hl".
+    wp_send with "[$HIxv]". wp_apply ("IH" with "Hl Hc HI"). by rewrite -assoc_L.
   Qed.
 
   Lemma recv_all_spec c p xs ys' :
     Sorted R ys' →
     {{{ c ↣ sort_elem_tail_protocol I R xs ys' <++> p @ N }}}
       recv_all c
-    {{{ ys ws, RET (llist ws);
+    {{{ l ys ws, RET #l;
         ⌜Sorted R (ys' ++ ys)⌝ ∗ ⌜ys' ++ ys ≡ₚ xs⌝ ∗
-        c ↣ p @ N ∗ [∗ list] y;w ∈ ys;ws, I y w
+        llist l ws ∗ c ↣ p @ N ∗ [∗ list] y;w ∈ ys;ws, I y w
     }}}.
   Proof.
     iIntros (Hsort Φ) "Hc HΦ".
@@ -57,30 +56,32 @@ Section sort_elem_client.
     wp_lam. wp_branch as %_ | %Hperm; wp_pures.
     - wp_recv (y v) as (Htl) "HIxv".
       wp_apply ("IH" with "[] Hc"); first by auto using Sorted_snoc.
-      iIntros (ys ws). rewrite -!assoc_L. iDestruct 1 as (??) "[Hc HI]".
-      wp_apply (lcons_spec with "[//]"); iIntros (_).
-      iApply ("HΦ" $! (y :: ys)). simpl; iFrame; auto.
-    - wp_apply (lnil_spec with "[//]"); iIntros (_).
-      iApply ("HΦ" $! [] []); rewrite /= right_id_L; by iFrame.
+      iIntros (l ys ws). rewrite -!assoc_L. iDestruct 1 as (??) "(Hl & Hc & HI)".
+      wp_apply (lcons_spec with "Hl"); iIntros "Hl".
+      iApply ("HΦ" $! _ (y :: ys)); simpl; eauto with iFrame.
+    - wp_apply (lnil_spec with "[//]"); iIntros (l) "Hl".
+      iApply ("HΦ" $! _ [] []); rewrite /= right_id_L; by iFrame.
   Qed.
 
-  Lemma sort_client_spec cmp vs xs :
+  Lemma sort_client_spec cmp l vs xs :
     cmp_spec I R cmp -∗
-    {{{ [∗ list] x;v ∈ xs;vs, I x v }}}
-      sort_elem_client cmp (llist vs)
-    {{{ ys ws, RET (llist ws); ⌜Sorted R ys⌝ ∗ ⌜ys ≡ₚ xs⌝ ∗
-               [∗ list] y;w ∈ ys;ws, I y w }}}.
+    {{{ llist l vs ∗ [∗ list] x;v ∈ xs;vs, I x v }}}
+      sort_elem_client cmp #l
+    {{{ k ys ws, RET #k;
+        ⌜Sorted R ys⌝ ∗ ⌜ys ≡ₚ xs⌝ ∗
+        llist k ws ∗ [∗ list] y;w ∈ ys;ws, I y w
+    }}}.
   Proof.
-    iIntros "#Hcmp !>" (Φ) "HI HΦ". wp_lam.
+    iIntros "#Hcmp !>" (Φ) "[Hl HI] HΦ". wp_lam.
     wp_apply (start_chan_proto_spec N (sort_elem_top_protocol <++> END)%proto);
       iIntros (c) "Hc".
     { wp_apply (sort_elem_service_top_spec N with "Hc"); auto. }
     rewrite /sort_elem_top_protocol.
     wp_send (A I R) with "[$Hcmp]".
-    wp_apply (send_all_spec with "[$HI $Hc]"); iIntros "Hc".
+    wp_apply (send_all_spec with "[$Hl $HI $Hc]"); iIntros "Hc".
     wp_select.
     wp_apply (recv_all_spec _ _ _ [] with "[$Hc]"); auto.
-    iIntros (ys ws) "/=". iDestruct 1 as (??) "[_ HI]".
-    iApply "HΦ"; auto.
+    iIntros (k ys ws) "/=". iDestruct 1 as (??) "(Hk & _ & HI)".
+    iApply "HΦ"; auto with iFrame.
   Qed.
 End sort_elem_client.
