theories/examples/sort_elem.v
@@ -2,7 +2,7 @@ From stdpp Require Import sorting.
 From actris.channel Require Import proto_channel proofmode.
 From iris.heap_lang Require Import proofmode notation.
 From iris.heap_lang Require Import assert.
-From actris.utils Require Import list compare.
+From actris.utils Require Import compare.
 
 Definition cont := true.
 Definition stop := false.
